Median and merge sort changes

statistics.dfy
@@ -1,123 +1,106 @@
 module Statistics {
 
-  function Sum(s: seq<real>) : real
-    decreases |s|
-  {
-    if |s| == 0 then 0.0 else s[0] + Sum(s[1..])
-  }
-
-  function Mean(s: seq<real>) : real
-    requires |s| > 0
-  {
-    Sum(s) / (|s| as real)
-  }
-
+  
   predicate Sorted(s: seq<real>)
   {
     forall i :: 0 <= i && i + 1 < |s| ==> s[i] <= s[i+1]
   }
-
-  function Merge(left: seq<real>, right: seq<real>) : seq<real>
-    decreases |left| + |right|
+ // This is the join function which combines the 2 sorted parts
+  function merge_join(first: seq<real>, second: seq<real>) : seq<real>
+    decreases |first| + |second|
   {
-    if |left| == 0 then right
-    else if |right| == 0 then left
-    else if left[0] <= right[0]
-         then [left[0]] + Merge(left[1..], right)
-         else [right[0]] + Merge(left, right[1..])
+    if |first| == 0 then second
+    else if |second| == 0 then first
+    else if first[0] <= second[0]
+         then [first[0]] + merge_join(first[1..], second)
+         else [second[0]] + merge_join(first, second[1..])
   }
-
-  function MergeSort(s: seq<real>) : seq<real>
+// This is the split function which splits the sequence into 2 parts
+  function merge_split(s: seq<real>) : seq<real>
     decreases |s|
   {
     if |s| <= 1 then s
     else
       var mid := |s| / 2;
-      Merge(MergeSort(s[..mid]), MergeSort(s[mid..]))
+      merge_join(merge_split(s[..mid]), merge_split(s[mid..]))
   }
 
-  lemma Merge_Length(left: seq<real>, right: seq<real>)
-    ensures |Merge(left,right)| == |left| + |right|
-    decreases |left| + |right|
+  lemma merge_join_Length(first: seq<real>, second: seq<real>)
+    ensures |merge_join(first,second)| == |first| + |second|
+    decreases |first| + |second|
   {
-    if |left| == 0 || |right| == 0 { }
-    else if left[0] <= right[0] {
-      Merge_Length(left[1..], right);
+    if |first| == 0 || |second| == 0 { }
+    else if first[0] <= second[0] {
+      merge_join_Length(first[1..], second);
     } else {
-      Merge_Length(left, right[1..]);
+      merge_join_Length(first, second[1..]);
     }
   }
 
-  lemma MergeSort_Length(s: seq<real>)
-    ensures |MergeSort(s)| == |s|
+  lemma merge_split_Length(s: seq<real>)
+    ensures |merge_split(s)| == |s|
     decreases |s|
   {
     if |s| <= 1 { }
     else {
       var mid := |s| / 2;
-      MergeSort_Length(s[..mid]);
-      MergeSort_Length(s[mid..]);
-      Merge_Length(MergeSort(s[..mid]), MergeSort(s[mid..]));
+      merge_split_Length(s[..mid]);
+      merge_split_Length(s[mid..]);
+      merge_join_Length(merge_split(s[..mid]), merge_split(s[mid..]));
     }
   }
 
-  lemma Merge_Sorted(left: seq<real>, right: seq<real>)
-    requires Sorted(left) && Sorted(right)
-    ensures Sorted(Merge(left,right))
-    decreases |left| + |right|
+  lemma merge_join_sorted(first: seq<real>, second: seq<real>)
+    requires Sorted(first) && Sorted(second)
+    ensures Sorted(merge_join(first,second))
+    decreases |first| + |second|
   {
-    if |left| == 0 || |right| == 0 {
-    } else if left[0] <= right[0] {
-      Merge_Sorted(left[1..], right);
-      if |left| >= 2 {
-        assert left[0] <= left[1];
+    if |first| == 0 || |second| == 0 {
+    } else if first[0] <= second[0] {
+      merge_join_sorted(first[1..], second);
+      if |first| >= 2 {
+        assert first[0] <= first[1];
       } else {
-        assert left[0] <= right[0];
+        assert first[0] <= second[0];
       }
     } else {
-      Merge_Sorted(left, right[1..]);
-      if |right| >= 2 {
-        assert right[0] <= right[1];
+      merge_join_sorted(first, second[1..]);
+      if |second| >= 2 {
+        assert second[0] <= second[1];
       } else {
-        assert right[0] <= left[0];
+        assert second[0] <= first[0];
       }
     }
   }
 
-  lemma MergeSort_Sorted(s: seq<real>)
-    ensures Sorted(MergeSort(s))
+  lemma merge_split_Sorted(s: seq<real>)
+    ensures Sorted(merge_split(s))
     decreases |s|
   {
     if |s| <= 1 { }
     else {
       var mid := |s| / 2;
-      MergeSort_Sorted(s[..mid]);
-      MergeSort_Sorted(s[mid..]);
-      Merge_Sorted(MergeSort(s[..mid]), MergeSort(s[mid..]));
+      merge_split_Sorted(s[..mid]);
+      merge_split_Sorted(s[mid..]);
+      merge_join_sorted(merge_split(s[..mid]), merge_split(s[mid..]));
     }
   }
 
-  lemma EvenPositiveImpliesAtLeastTwo(n: nat)
-    requires n > 0 && n % 2 == 0
-    ensures n >= 2
-  { }
+  
 
   method Median(s: seq<real>) returns (m: real)
-    requires |s| > 0
-    ensures if |MergeSort(s)| % 2 == 1
-            then m == MergeSort(s)[|MergeSort(s)|/2]
-            else m == (MergeSort(s)[|MergeSort(s)|/2 - 1] + MergeSort(s)[|MergeSort(s)|/2]) / 2.0
-  {
-    var t := MergeSort(s);
-    MergeSort_Length(s);
-    if |t| % 2 == 1 {
-      m := t[|t|/2];
-      assert m == MergeSort(s)[|MergeSort(s)|/2];
-    } else {
-      assert |t| > 0;
-      EvenPositiveImpliesAtLeastTwo(|t| as nat);
-      m := (t[|t|/2 - 1] + t[|t|/2]) / 2.0;
-      assert m == (MergeSort(s)[|MergeSort(s)|/2 - 1] + MergeSort(s)[|MergeSort(s)|/2]) / 2.0;
-    }
+  requires |s| > 0
+  ensures (|merge_split(s)| % 2 == 1 ==> 
+             m == merge_split(s)[|merge_split(s)|/2])
+  ensures (|merge_split(s)| % 2 == 0 && |merge_split(s)| >= 2 ==> 
+             m == (merge_split(s)[|merge_split(s)|/2 - 1] + merge_split(s)[|merge_split(s)|/2]) / 2.0)
+{
+  var t := merge_split(s);
+ merge_split_Length(s);                         
+  if |t| % 2 == 1 {
+    m := t[|t|/2];
+  } else {
+    m := (t[|t|/2 - 1] + t[|t|/2]) / 2.0;
   }
+}
 }
