test_stat.dfy
@@ -3,44 +3,32 @@ include "statistics.dfy"
 module TestStatistics {
   import opened Statistics
 
-  method {:test} TestSum() {
-    assert Sum([]) == 0.0;
-    assert Sum([1.0, 2.0, 3.0]) == 6.0;
-    assert Sum([-5.0, 0.0, 10.0]) == 5.0;
-  }
 
-  method {:test} TestMean() {
-    assert Mean([42.0]) == 42.0;
-    assert Mean([2.0, 4.0, 6.0, 8.0]) == 5.0;
-    assert Mean([1.5, 2.5, 3.5]) == 2.5;
-  }
-
-  method {:test} TestMedianByDefinition_Odd() {
+  method {:test} test_median_Odd() {
     var s := [3.0, 1.0, 2.0];
     var m: real;
     m := Median(s);
-    MergeSort_Length(s);
-    var t := MergeSort(s);
+    merge_split_Length(s);
+    var t := merge_split(s);
     assert m == t[|t|/2];
   }
 
-  method {:test} TestMedianByDefinition_Even() {
+  method {:test} test_median_Even() {
     var s := [4.0, 1.0, 2.0, 3.0];
     var m: real;
     m := Median(s);
-    MergeSort_Length(s);
-    var t := MergeSort(s);
+    merge_split_Length(s);
+    var t := merge_split(s);
     assert |t| % 2 == 0;
-    EvenPositiveImpliesAtLeastTwo(|t| as nat);
     assert m == (t[|t|/2 - 1] + t[|t|/2]) / 2.0;
   }
 
-  method {:test} TestMedianNegatives_ByDefinition() {
+  method {:test} test_median_negative() {
     var s := [-5.0, -1.0, -3.0];
     var m: real;
     m := Median(s);
-    MergeSort_Length(s);
-    var t := MergeSort(s);
+    merge_split_Length(s);
+    var t := merge_split(s);
     assert m == t[|t|/2];
   }
 }
